\documentclass{article}
\usepackage[utf8]{inputenc}

\usepackage[T2A]{fontenc}
\usepackage[utf8]{inputenc}
\usepackage[russian]{babel}

\usepackage{amsmath}

\usepackage{pgfplots}
\usepackage{sagetex}
\usepgfplotslibrary{fillbetween}
\usepgfplotslibrary{polar}
\pgfplotsset{compat=newest}

\usepackage{multienum}
\usepackage{geometry}
\geometry{
    left=1cm,right=1cm,top=2cm,bottom=2cm
}
\newcommand*\diff{\mathop{}\!\mathrm{d}}

\newtheorem{definition}{Определение}
\newtheorem{theorem}{Теорема}

\DeclareMathOperator{\sign}{sign}

\usepackage{hyperref}
\hypersetup{
    colorlinks, citecolor=black, filecolor=black, linkcolor=black, urlcolor=black
}

\title{Высшая математика}
\author{Лисид Лаконский}
\date{May 2023}

\begin{document}
\raggedright

\maketitle

\tableofcontents
\pagebreak

\section{Действия с комплексными числами, вариант №21}

\subsection{Задание №1}

Вычислить $a + b$, $a b$, $a / b$, если

$$
a = 3 + 3 i, \ b = 2 - i
$$

\textbf{Решение.}

\begin{enumerate}
    \item $a = 3 + 3 i$, $b = 2 - i$ \\
    $a + b = (3 + 3 i) + (2 - i) = 5 + 2 i$ \\
    $ab = (3 + 3 i) (2 - i) = 6 - 3i + 6i - 3 i^2 = 9 + 3 i $ \\
    $\frac{a}{b} = \frac{3 + 3 i}{2 - i} = \frac{(3 + 3 i)(2 + i)}{(2 - i)(2 + i)} = \frac{6 + 3 i + 6 i + 3 i^2}{2^2 - i^2} = \frac{3 + 9i}{5} = \frac{3}{5} + \frac{9 i}{5}$
\end{enumerate}

\textbf{Ответ:} см. выше

\subsection{Задание №2}

Найти все значения корня

$$
\sqrt[4]{\frac{1}{16}}
$$

\textbf{Решение.}

$\sqrt[4]{\frac{1}{16}} = \frac{1}{2}$, $\sqrt[4]{\frac{1}{16}} = -\frac{1}{2}$, $\sqrt[4]{\frac{1}{16}} = \frac{1 i}{2}$, $\sqrt[4]{\frac{1}{16}} = - \frac{1 i}{2}$

\hfill

\textbf{Ответ:} $\frac{1}{2}$, $-\frac{1}{2}$, $\frac{i}{2}$, $-\frac{i}{2}$

\subsection{Задание №3}

Вычислить

$$
(\frac{1 + i}{\sqrt{2}})^{2 i}
$$

\textbf{Решение.}

$(\frac{1 + i}{\sqrt{2}})^{2 i} = e^{(2 i) Ln (\frac{1}{\sqrt{2}} + \frac{i}{\sqrt{2}})} = e^{(2 i) (\ln \sqrt{\frac{1}{4}} + i (\arctg 1 + 2 \pi n))} = e^{(2 i) (\ln \sqrt{\frac{1}{4}} + i (\frac{\pi}{4} + 2 \pi n))}$

\hfill

\textbf{Ответ:} $e^{(2 i) (\ln \sqrt{\frac{1}{4}} + i (\frac{\pi}{4} + 2 \pi n))}$

\end{document}